cleanup

Saturation_Framework/Ordered_Resolution_Integration.thy
@@ -1,8 +1,8 @@
-(*  Title:       Ordered_Resolution_Integration
+(*  Title:       Application of the Saturation Framework to Bachmair and Ganzinger's RP
  *  Author:      Sophie Tourret <stourret at mpi-inf.mpg.de>, 2018-2020
  *  Author:      Jasmin Blanchette <j.c.blanchette at vu.nl>, 2020 *)
 
-section \<open>Application of the saturation framework to Bachmair and Ganzinger's RP\<close>
+section \<open>Application of the Saturation Framework to Bachmair and Ganzinger's RP\<close>
 
 theory Ordered_Resolution_Integration
   imports
@@ -11,6 +11,10 @@ theory Ordered_Resolution_Integration
     Clausal_Inference_Systems
     Soundness
 begin
+
+text \<open>The main results about Bachmair and Ganzinger's RP prover, as established in Section 4.3 of
+their \emph{Handbook} chapter and formalized by Schlichtkrull et al., are reproved here using
+the saturation framework of Waldmann et al.\<close>
 
 
 subsection \<open>Setup\<close>
@@ -26,30 +30,30 @@ hide_const (open) Inference_System.Infer Inference_System.main_prem_of
   Inference_System.side_prems_of Inference_System.prems_of Inference_System.concl_of
   Inference_System.concls_of Inference_System.infer_from
 
-type_synonym 'a inference_RP = "'a Inference_System.inference"
+type_synonym 'a old_inference = "'a Inference_System.inference"
 
-abbreviation Infer_RP :: "'a clause multiset \<Rightarrow> 'a clause \<Rightarrow> 'a clause \<Rightarrow> 'a inference_RP" where
-  "Infer_RP \<equiv> Inference_System.Infer"
+abbreviation old_Infer :: "'a clause multiset \<Rightarrow> 'a clause \<Rightarrow> 'a clause \<Rightarrow> 'a old_inference" where
+  "old_Infer \<equiv> Inference_System.Infer"
 
-abbreviation side_prems_of_RP :: "'a inference_RP \<Rightarrow> 'a clause multiset" where
-  "side_prems_of_RP \<equiv> Inference_System.side_prems_of"
+abbreviation old_side_prems_of :: "'a old_inference \<Rightarrow> 'a clause multiset" where
+  "old_side_prems_of \<equiv> Inference_System.side_prems_of"
 
-abbreviation main_prem_of_RP :: "'a inference_RP \<Rightarrow> 'a clause" where
-  "main_prem_of_RP \<equiv> Inference_System.main_prem_of"
+abbreviation old_main_prem_of :: "'a old_inference \<Rightarrow> 'a clause" where
+  "old_main_prem_of \<equiv> Inference_System.main_prem_of"
 
-abbreviation concl_of_RP :: "'a inference_RP \<Rightarrow> 'a clause" where
-  "concl_of_RP \<equiv> Inference_System.concl_of"
+abbreviation old_concl_of :: "'a old_inference \<Rightarrow> 'a clause" where
+  "old_concl_of \<equiv> Inference_System.concl_of"
 
-abbreviation prems_of_RP :: "'a inference_RP \<Rightarrow> 'a clause multiset" where
-  "prems_of_RP \<equiv> Inference_System.prems_of"
+abbreviation old_prems_of :: "'a old_inference \<Rightarrow> 'a clause multiset" where
+  "old_prems_of \<equiv> Inference_System.prems_of"
 
-abbreviation concls_of_RP :: "'a inference_RP set \<Rightarrow> 'a clause set" where
-  "concls_of_RP \<equiv> Inference_System.concls_of"
+abbreviation old_concls_of :: "'a old_inference set \<Rightarrow> 'a clause set" where
+  "old_concls_of \<equiv> Inference_System.concls_of"
 
-abbreviation infer_from_RP :: "'a clause set \<Rightarrow> 'a inference_RP \<Rightarrow> bool" where
-  "infer_from_RP \<equiv> Inference_System.infer_from"
+abbreviation old_infer_from :: "'a clause set \<Rightarrow> 'a old_inference \<Rightarrow> bool" where
+  "old_infer_from \<equiv> Inference_System.infer_from"
 
-lemmas infer_from_RP_def = Inference_System.infer_from_def
+lemmas old_infer_from_def = Inference_System.infer_from_def
 
 
 subsection \<open>Library\<close>
@@ -57,13 +61,6 @@ subsection \<open>Library\<close>
 lemma set_zip_replicate_right[simp]:
   "set (zip xs (replicate (length xs) y)) = (\<lambda>x. (x, y)) ` set xs"
   by (induct xs) auto
-
-lemma po_on_empty_rel[simp]: "po_on (\<lambda>_ _. False) UNIV"
-  unfolding po_on_def irreflp_on_def transp_on_def by auto
-
-(* FIXME: needed? *)
-lemma (in substitution) union_grounding_of_cls_ground: "is_ground_clss (\<Union> (grounding_of_cls ` N))"
-  by (simp add: grounding_ground grounding_of_clss_def is_ground_clss_def)
 
 
 subsection \<open>Ground Layer\<close>
@@ -74,19 +71,19 @@ begin
 interpretation gr: ground_resolution_with_selection "S_M S M"
   using selection_axioms by unfold_locales (fact S_M_selects_subseteq S_M_selects_neg_lits)+
 
-definition Inf_G :: "'a clause set \<Rightarrow> 'a clause inference set" where
-  "Inf_G M = {Infer (CAs @ [DA]) E |CAs DA AAs As E. gr.ord_resolve M CAs DA AAs As E}"
+definition G_Inf :: "'a clause set \<Rightarrow> 'a clause inference set" where
+  "G_Inf M = {Infer (CAs @ [DA]) E |CAs DA AAs As E. gr.ord_resolve M CAs DA AAs As E}"
 
-lemma Inf_G_have_prems: "\<iota> \<in> Inf_G M \<Longrightarrow> prems_of \<iota> \<noteq> []"
-  unfolding Inf_G_def by auto
+lemma G_Inf_have_prems: "\<iota> \<in> G_Inf M \<Longrightarrow> prems_of \<iota> \<noteq> []"
+  unfolding G_Inf_def by auto
 
-lemma Inf_G_reductive: "\<iota> \<in> Inf_G M \<Longrightarrow> concl_of \<iota> < main_prem_of \<iota>"
-  unfolding Inf_G_def by (auto dest: gr.ord_resolve_reductive)
+lemma G_Inf_reductive: "\<iota> \<in> G_Inf M \<Longrightarrow> concl_of \<iota> < main_prem_of \<iota>"
+  unfolding G_Inf_def by (auto dest: gr.ord_resolve_reductive)
 
-interpretation G: sound_inference_system "Inf_G M" "{{#}}" "(\<TTurnstile>e)"
+interpretation G: sound_inference_system "G_Inf M" "{{#}}" "(\<TTurnstile>e)"
 proof
   fix \<iota>
-  assume i_in: "\<iota> \<in> Inf_G M"
+  assume i_in: "\<iota> \<in> G_Inf M"
   moreover
   {
     fix I
@@ -94,17 +91,17 @@ proof
     obtain CAs AAs As where
       the_inf: "gr.ord_resolve M CAs (main_prem_of \<iota>) AAs As (concl_of \<iota>)" and
       CAs: "CAs = side_prems_of \<iota>"
-      using i_in unfolding Inf_G_def by auto
+      using i_in unfolding G_Inf_def by auto
     then have "I \<TTurnstile> concl_of \<iota>"
       using gr.ord_resolve_sound[of M CAs "main_prem_of \<iota>" AAs As "concl_of \<iota>" I]
-      by (metis I_ent_prems Inf_G_have_prems i_in insert_is_Un set_mset_mset set_prems_of
+      by (metis I_ent_prems G_Inf_have_prems i_in insert_is_Un set_mset_mset set_prems_of
           true_clss_insert true_clss_set_mset)
   }
   ultimately show "set (inference.prems_of \<iota>) \<TTurnstile>e {concl_of \<iota>}"
     by simp
 qed
 
-interpretation G: clausal_cex_red_inference_system "Inf_G M" "gr.INTERP M"
+interpretation G: clausal_cex_red_inference_system "G_Inf M" "gr.INTERP M"
 proof
   fix N D
   assume
@@ -120,19 +117,16 @@ proof
     "\<not> gr.INTERP M N \<TTurnstile> E" and
     "E < D"
     using gr.ord_resolve_counterex_reducing by blast
-  then show "\<exists>Cs E. set Cs \<subseteq> N \<and> gr.INTERP M N \<TTurnstile>s set Cs \<and> Infer (Cs @ [D]) E \<in> Inf_G M
+  then show "\<exists>Cs E. set Cs \<subseteq> N \<and> gr.INTERP M N \<TTurnstile>s set Cs \<and> Infer (Cs @ [D]) E \<in> G_Inf M
     \<and> \<not> gr.INTERP M N \<TTurnstile> E \<and> E < D"
-    unfolding Inf_G_def
+    unfolding G_Inf_def
     by (metis (mono_tags, lifting) gr.ex_min_counterex gr.productive_imp_INTERP mem_Collect_eq)
 qed
 
-interpretation G: clausal_cex_red_calculus_with_std_red_crit "Inf_G M" "gr.INTERP M"
-  by (unfold_locales, fact Inf_G_have_prems, fact Inf_G_reductive)
+interpretation G: clausal_cex_red_calculus_with_std_red_crit "G_Inf M" "gr.INTERP M"
+  by (unfold_locales, fact G_Inf_have_prems, fact G_Inf_reductive)
 
-abbreviation derive_G (infix "\<rhd>RedG" 50) where
-  "(\<rhd>RedG) \<equiv> G.derive"
-
-interpretation G: static_refutational_complete_calculus "{{#}}" "Inf_G M" "(\<TTurnstile>e)" "G.Red_Inf M"
+interpretation G: static_refutational_complete_calculus "{{#}}" "G_Inf M" "(\<TTurnstile>e)" "G.Red_Inf M"
   G.Red_F
   by unfold_locales (use G.clausal_saturated_complete in blast)
 
@@ -142,23 +136,29 @@ subsection \<open>First-Order Layer\<close>
 abbreviation \<G>_F :: \<open>'a clause \<Rightarrow> 'a clause set\<close> where
   \<open>\<G>_F \<equiv> grounding_of_cls\<close>
 
+abbreviation \<G>_Fs :: \<open>'a clause set \<Rightarrow> 'a clause set\<close> where
+  \<open>\<G>_Fs \<equiv> grounding_of_clss\<close>
+
 lemmas \<G>_F_def = grounding_of_cls_def
+lemmas \<G>_Fs_def = grounding_of_clss_def
 
 definition \<G>_Inf :: \<open>'a clause set \<Rightarrow> 'a clause inference \<Rightarrow> 'a clause inference set\<close> where
   \<open>\<G>_Inf M \<iota> = {Infer (prems_of \<iota> \<cdot>\<cdot>cl \<rho>s) (concl_of \<iota> \<cdot> \<rho>) |\<rho> \<rho>s.
      is_ground_subst_list \<rho>s \<and> is_ground_subst \<rho>
-     \<and> Infer (prems_of \<iota> \<cdot>\<cdot>cl \<rho>s) (concl_of \<iota> \<cdot> \<rho>) \<in> Inf_G M}\<close>
+     \<and> Infer (prems_of \<iota> \<cdot>\<cdot>cl \<rho>s) (concl_of \<iota> \<cdot> \<rho>) \<in> G_Inf M}\<close>
 
-abbreviation \<G>_Inf_opt :: \<open>'a clause set \<Rightarrow> 'a clause inference \<Rightarrow> 'a clause inference set option\<close> where
+abbreviation
+  \<G>_Inf_opt :: \<open>'a clause set \<Rightarrow> 'a clause inference \<Rightarrow> 'a clause inference set option\<close>
+where
   \<open>\<G>_Inf_opt M \<iota> \<equiv> Some (\<G>_Inf M \<iota>)\<close>
 
-definition Inf_F :: "'a clause inference set" where
-  "Inf_F = {Infer (CAs @ [DA]) E | CAs DA AAs As \<sigma> E. ord_resolve_rename S CAs DA AAs As \<sigma> E}"
+definition F_Inf :: "'a clause inference set" where
+  "F_Inf = {Infer (CAs @ [DA]) E | CAs DA AAs As \<sigma> E. ord_resolve_rename S CAs DA AAs As \<sigma> E}"
 
-lemma Inf_F_have_prems: "\<iota> \<in> Inf_F \<Longrightarrow> prems_of \<iota> \<noteq> []"
-  unfolding Inf_F_def by force
+lemma F_Inf_have_prems: "\<iota> \<in> F_Inf \<Longrightarrow> prems_of \<iota> \<noteq> []"
+  unfolding F_Inf_def by force
 
-interpretation F: standard_lifting_with_red_crit_family Inf_F "{{#}}" UNIV Inf_G "\<lambda>N. (\<TTurnstile>e)"
+interpretation F: standard_lifting_with_red_crit_family F_Inf "{{#}}" UNIV G_Inf "\<lambda>N. (\<TTurnstile>e)"
   G.Red_Inf "\<lambda>N. G.Red_F" "{{#}}" "\<lambda>N. \<G>_F" \<G>_Inf_opt "\<lambda>D C C'. False"
 proof (unfold_locales; (intro ballI)?)
   show "UNIV \<noteq> {}"
@@ -167,48 +167,36 @@ next
   show "consequence_relation {{#}} (\<TTurnstile>e)"
     by (fact consequence_relation_axioms)
 next
-  show "\<And>M. calculus_with_red_crit {{#}} (Inf_G M) (\<TTurnstile>e) (G.Red_Inf M) G.Red_F"
+  show "\<And>M. calculus_with_red_crit {{#}} (G_Inf M) (\<TTurnstile>e) (G.Red_Inf M) G.Red_F"
     by (fact G.calculus_with_red_crit_axioms)
 next
-  show "\<And>M. lifting_with_wf_ordering_family {{#}} Inf_F {{#}} (\<TTurnstile>e) (Inf_G M) (G.Red_Inf M)
+  show "\<And>M. lifting_with_wf_ordering_family {{#}} F_Inf {{#}} (\<TTurnstile>e) (G_Inf M) (G.Red_Inf M)
     G.Red_F \<G>_F (\<G>_Inf_opt M) (\<lambda>D C C'. False)"
-    unfolding lifting_with_wf_ordering_family_def standard_lifting_def standard_lifting_axioms_def
-  proof (intro allI impI conjI)
-    show "\<And>M. calculus_with_red_crit {{#}} (Inf_G M) (\<TTurnstile>e) (G.Red_Inf M) G.Red_F"
-      by (fact G.calculus_with_red_crit_axioms)
-  next
-    show "{{#}} \<noteq> {}"
-      by auto
-  next
-    fix B :: "'a clause"
-    assume "B \<in> {{#}}"
-    then show "\<G>_F B \<noteq> {}"
-      unfolding \<G>_F_def by (simp add: ex_ground_subst)
-  next
-    fix B :: "'a clause"
-    assume "B \<in> {{#}}"
-    then show "\<G>_F B \<subseteq> {{#}}"
-      unfolding \<G>_F_def using is_ground_cls_empty is_ground_subst_cls by blast
-  next
-    fix C
-    assume "\<G>_F C \<inter> {{#}} \<noteq> {}"
-    then show "C \<in> {{#}}"
-      unfolding \<G>_F_def by auto
-  next
+  proof
     fix M \<iota>
-    assume \<iota>_in: "\<iota> \<in> Inf_F"
+    assume \<iota>_in: "\<iota> \<in> F_Inf"
 
     show "the (\<G>_Inf_opt M \<iota>) \<subseteq> G.Red_Inf M (\<G>_F (concl_of \<iota>))"
-      unfolding \<G>_Inf_def G.Red_Inf_def G.redundant_infer_def
-      apply clarsimp
-      apply (rule_tac x = "{concl_of \<iota> \<cdot> \<rho>}" in exI)
-      unfolding \<G>_F_def
-      apply auto
-      using Inf_G_reductive by fastforce
-  next
-    show "lifting_with_wf_ordering_family_axioms (\<lambda>D C C'. False)"
-      unfolding lifting_with_wf_ordering_family_axioms_def minimal_element_def by simp
-  qed
+      unfolding option.sel
+    proof
+      fix \<iota>'
+      assume \<iota>'_in: "\<iota>' \<in> \<G>_Inf M \<iota>"
+      then obtain \<rho> \<rho>s where
+        \<iota>': "\<iota>' = Infer (prems_of \<iota> \<cdot>\<cdot>cl \<rho>s) (concl_of \<iota> \<cdot> \<rho>)" and
+        \<rho>s_gr: "is_ground_subst_list \<rho>s" and
+        \<rho>_gr: "is_ground_subst \<rho>" and
+        \<rho>_infer: "Infer (prems_of \<iota> \<cdot>\<cdot>cl \<rho>s) (concl_of \<iota> \<cdot> \<rho>) \<in> G_Inf M"
+        unfolding \<G>_Inf_def by blast
+
+      let ?DD1 = "{concl_of \<iota> \<cdot> \<rho>}"
+
+      show "\<iota>' \<in> G.Red_Inf M (\<G>_F (concl_of \<iota>))"
+        unfolding G.Red_Inf_def G.redundant_infer_def mem_Collect_eq using \<iota>' \<rho>_gr \<rho>_infer
+        by (metis inference.sel(2) G_Inf_reductive empty_iff ground_subst_ground_cls
+            grounding_of_cls_ground insert_iff subst_cls_eq_grounding_of_cls_subset_eq
+            true_clss_union)
+    qed
+  qed (auto simp: \<G>_F_def ex_ground_subst)
 qed
 
 notation F.entails_\<G>_Q (infix "\<TTurnstile>\<G>e" 50)
@@ -220,10 +208,10 @@ lemma true_Union_grounding_of_cls_iff_true_all_interps_ground_substs:
   "I \<TTurnstile>s (\<Union>C \<in> N. {C \<cdot> \<sigma> |\<sigma>. is_ground_subst \<sigma>}) \<longleftrightarrow> (\<forall>\<sigma>. is_ground_subst \<sigma> \<longrightarrow> I \<TTurnstile>s N \<cdot>cs \<sigma>)"
   unfolding true_clss_def subst_clss_def by blast
 
-interpretation F: sound_inference_system Inf_F "{{#}}" "(\<TTurnstile>\<G>e)"
+interpretation F: sound_inference_system F_Inf "{{#}}" "(\<TTurnstile>\<G>e)"
 proof
   fix \<iota>
-  assume i_in: "\<iota> \<in> Inf_F"
+  assume i_in: "\<iota> \<in> F_Inf"
   moreover
   {
     fix I \<eta>
@@ -233,9 +221,9 @@ proof
     obtain CAs AAs As \<sigma> where
       the_inf: "ord_resolve_rename S CAs (main_prem_of \<iota>) AAs As \<sigma> (concl_of \<iota>)" and
       CAs: "CAs = side_prems_of \<iota>"
-      using i_in unfolding Inf_F_def by auto
+      using i_in unfolding F_Inf_def by auto
     have prems: "mset (prems_of \<iota>) = mset (side_prems_of \<iota>) + {#main_prem_of \<iota>#}"
-      by (metis (no_types) Inf_F_have_prems[OF i_in] add.right_neutral append_Cons append_Nil2
+      by (metis (no_types) F_Inf_have_prems[OF i_in] add.right_neutral append_Cons append_Nil2
           append_butlast_last_id mset.simps(2) mset_rev mset_single_iff_right rev_append
           rev_is_Nil_conv union_mset_add_mset_right)
     have "I \<TTurnstile> concl_of \<iota> \<cdot> \<eta>"
@@ -255,12 +243,12 @@ proof -
   assume \<iota>\<^sub>0_in: "\<iota>\<^sub>0 \<in> G.Inf_from M (\<Union> (\<G>_F ` M))"
   have prems_\<iota>\<^sub>0_in: "set (prems_of \<iota>\<^sub>0) \<subseteq> \<Union> (\<G>_F ` M)"
     using \<iota>\<^sub>0_in unfolding G.Inf_from_def by simp
-  have \<iota>\<^sub>0_Inf_G: \<open>\<iota>\<^sub>0 \<in> Inf_G M\<close>
+  have \<iota>\<^sub>0_G_Inf: \<open>\<iota>\<^sub>0 \<in> G_Inf M\<close>
     using \<iota>\<^sub>0_in unfolding G.Inf_from_def inference_system.Inf_from_def by blast
   then obtain CAs DA AAs As E where
     gr_res: \<open>gr.ord_resolve M CAs DA AAs As E\<close> and
     \<iota>\<^sub>0_is: \<open>\<iota>\<^sub>0 = Infer (CAs @ [DA]) E\<close>
-    unfolding Inf_G_def by auto
+    unfolding G_Inf_def by auto
 
   have CAs_in: \<open>set CAs \<subseteq> set (prems_of \<iota>\<^sub>0)\<close>
     by (simp add: \<iota>\<^sub>0_is subsetI)
@@ -274,8 +262,8 @@ proof -
     grounded_res: \<open>ord_resolve (S_M S M) CAs DA AAs As \<sigma> E\<close>
     using ground_ord_resolve_imp_ord_resolve[OF ground_DA ground_CAs
         gr.ground_resolution_with_selection_axioms gr_res] by auto
-  have prems_ground: \<open>{DA} \<union> set CAs \<subseteq> grounding_of_clss M\<close>
-    using prems_\<iota>\<^sub>0_in CAs_in DA_in unfolding grounding_of_clss_def by fast
+  have prems_ground: \<open>{DA} \<union> set CAs \<subseteq> \<G>_Fs M\<close>
+    using prems_\<iota>\<^sub>0_in CAs_in DA_in unfolding \<G>_Fs_def by fast
 
   obtain \<eta>s \<eta> \<eta>2 CAs0 DA0 AAs0 As0 E0 \<tau> where
     ground_n: "is_ground_subst \<eta>" and
@@ -299,89 +287,72 @@ proof -
   define \<iota> :: "'a clause inference" where
     "\<iota> = Infer (CAs0 @ [DA0]) E0"
 
-  have i_Inf_F: \<open>\<iota> \<in> Inf_F\<close>
-    unfolding \<iota>_def Inf_F_def using ngr_res by auto
+  have i_F_Inf: \<open>\<iota> \<in> F_Inf\<close>
+    unfolding \<iota>_def F_Inf_def using ngr_res by auto
 
   have "\<exists>\<rho> \<rho>s. \<iota>\<^sub>0 = Infer ((CAs0 @ [DA0]) \<cdot>\<cdot>cl \<rho>s) (E0 \<cdot> \<rho>) \<and> is_ground_subst_list \<rho>s
-    \<and> is_ground_subst \<rho> \<and> Infer ((CAs0 @ [DA0]) \<cdot>\<cdot>cl \<rho>s) (E0 \<cdot> \<rho>) \<in> Inf_G M"
+    \<and> is_ground_subst \<rho> \<and> Infer ((CAs0 @ [DA0]) \<cdot>\<cdot>cl \<rho>s) (E0 \<cdot> \<rho>) \<in> G_Inf M"
     by (rule exI[of _ \<eta>2], rule exI[of _ "\<eta>s @ [\<eta>]"], use ground_ns in
-        \<open>auto intro: ground_n ground_n2 \<iota>\<^sub>0_Inf_G[unfolded \<iota>\<^sub>0_is']
+        \<open>auto intro: ground_n ground_n2 \<iota>\<^sub>0_G_Inf[unfolded \<iota>\<^sub>0_is']
            simp: \<iota>\<^sub>0_is' is_ground_subst_list_def\<close>)
   then have \<open>\<iota>\<^sub>0 \<in> \<G>_Inf M \<iota>\<close>
     unfolding \<G>_Inf_def \<iota>_def CAs0_is[symmetric] DA0_is[symmetric] E0_is[symmetric] by simp
   moreover have \<open>\<iota> \<in> F.Inf_from M\<close>
-    using prems_in i_Inf_F unfolding F.Inf_from_def \<iota>_def by simp
+    using prems_in i_F_Inf unfolding F.Inf_from_def \<iota>_def by simp
   ultimately show ?thesis
     by blast
 qed
 
-interpretation F: static_refutational_complete_calculus "{{#}}" Inf_F "(\<TTurnstile>\<G>e)" F.Red_Inf_\<G>_Q
+interpretation F: static_refutational_complete_calculus "{{#}}" F_Inf "(\<TTurnstile>\<G>e)" F.Red_Inf_\<G>_Q
   F.Red_F_\<G>_empty
-proof (rule F.stat_ref_comp_to_non_ground_fam_inter; clarsimp)
-  show "\<And>M. static_refutational_complete_calculus {{#}} (Inf_G M) (\<TTurnstile>e) (G.Red_Inf M) G.Red_F"
+proof (rule F.stat_ref_comp_to_non_ground_fam_inter; clarsimp; (intro exI)?)
+  show "\<And>M. static_refutational_complete_calculus {{#}} (G_Inf M) (\<TTurnstile>e) (G.Red_Inf M) G.Red_F"
     by (fact G.static_refutational_complete_calculus_axioms)
 next
   fix N
   assume "F.saturated N"
-  show "\<exists>M. F.ground.Inf_from_q M (\<Union> (\<G>_F ` N)) \<subseteq> {\<iota>. \<exists>\<iota>' \<in> F.Inf_from N. \<iota> \<in> \<G>_Inf M \<iota>'}
-    \<union> G.Red_Inf M (\<Union> (\<G>_F ` N))"
-    using G_Inf_overapproximates_F_Inf
-    apply auto
-    apply (rule exI[of _ N])
-    apply auto
-    using F.ground.Inf_from_q_def \<G>_Inf_def by fastforce
+  show "F.ground.Inf_from_q N (\<Union> (\<G>_F ` N)) \<subseteq> {\<iota>. \<exists>\<iota>' \<in> F.Inf_from N. \<iota> \<in> \<G>_Inf N \<iota>'}
+    \<union> G.Red_Inf N (\<Union> (\<G>_F ` N))"
+    using G_Inf_overapproximates_F_Inf unfolding F.ground.Inf_from_q_def \<G>_Inf_def by fastforce
 qed
 
 
-subsection \<open>Given Clause Layer\<close>
+subsection \<open>Labeled First-Order Layer (or Given Clause Layer)\<close>
 
 datatype label =
   New
 | Processed
 | Old
 
-definition Infer_FL_of :: "'a clause inference \<Rightarrow> ('a clause \<times> label) inference set" where
-  "Infer_FL_of \<iota> = {Infer Cls (D, New) |Cls D. \<iota> = Infer (map fst Cls) D}"
+definition FL_Infer_of :: "'a clause inference \<Rightarrow> ('a clause \<times> label) inference set" where
+  "FL_Infer_of \<iota> = {Infer Cls (D, New) |Cls D. \<iota> = Infer (map fst Cls) D}"
 
-definition Inf_FL :: "('a clause \<times> label) inference set" where
-  "Inf_FL = (\<Union>\<iota> \<in> Inf_F. Infer_FL_of \<iota>)"
+definition FL_Inf :: "('a clause \<times> label) inference set" where
+  "FL_Inf = (\<Union>\<iota> \<in> F_Inf. FL_Infer_of \<iota>)"
 
-abbreviation Equiv_F :: "'a clause \<Rightarrow> 'a clause \<Rightarrow> bool" (infix "\<doteq>" 50) where
+abbreviation F_Equiv :: "'a clause \<Rightarrow> 'a clause \<Rightarrow> bool" (infix "\<doteq>" 50) where
   "C \<doteq> D \<equiv> generalizes C D \<and> generalizes D C"
 
-abbreviation Prec_F :: "'a clause \<Rightarrow> 'a clause \<Rightarrow> bool" (infix "\<prec>\<cdot>" 50) where
+abbreviation F_Prec :: "'a clause \<Rightarrow> 'a clause \<Rightarrow> bool" (infix "\<prec>\<cdot>" 50) where
   "C \<prec>\<cdot> D \<equiv> strictly_generalizes C D"
 
-fun Prec_l :: "label \<Rightarrow> label \<Rightarrow> bool" (infix "\<sqsubset>l" 50) where
+fun L_Prec :: "label \<Rightarrow> label \<Rightarrow> bool" (infix "\<sqsubset>l" 50) where
   "Old \<sqsubset>l l \<longleftrightarrow> l \<noteq> Old"
 | "Processed \<sqsubset>l l \<longleftrightarrow> l = New"
 | "New \<sqsubset>l l \<longleftrightarrow> False"
 
-lemma irrefl_Prec_l: "\<not> l \<sqsubset>l l"
+lemma irrefl_L_Prec: "\<not> l \<sqsubset>l l"
   by (cases l) auto
 
-lemma trans_Prec_l: "l1 \<sqsubset>l l2 \<Longrightarrow> l2 \<sqsubset>l l3 \<Longrightarrow> l1 \<sqsubset>l l3"
+lemma trans_L_Prec: "l1 \<sqsubset>l l2 \<Longrightarrow> l2 \<sqsubset>l l3 \<Longrightarrow> l1 \<sqsubset>l l3"
   by (cases l1; cases l2; cases l3) auto
 
-lemma wf_Prec_l: "wfP (\<sqsubset>l)"
-  by (metis Prec_l.elims(2) Prec_l.simps(3) not_accp_down wfP_accp_iff)
+lemma wf_L_Prec: "wfP (\<sqsubset>l)"
+  by (metis L_Prec.elims(2) L_Prec.simps(3) not_accp_down wfP_accp_iff)
 
-(* TODO: Break down *)
-interpretation GC: Given_Clause "{{#}}" Inf_F "{{#}}" UNIV "\<lambda>N. (\<TTurnstile>e)" Inf_G G.Red_Inf
-  "\<lambda>N. G.Red_F" "\<lambda>N. \<G>_F" \<G>_Inf_opt Inf_FL "(\<doteq>)" "(\<prec>\<cdot>)" "(\<sqsubset>l)" Old
+interpretation FL: Given_Clause "{{#}}" F_Inf "{{#}}" UNIV "\<lambda>N. (\<TTurnstile>e)" G_Inf G.Red_Inf
+  "\<lambda>N. G.Red_F" "\<lambda>N. \<G>_F" \<G>_Inf_opt FL_Inf "(\<doteq>)" "(\<prec>\<cdot>)" "(\<sqsubset>l)" Old
 proof (unfold_locales; (intro ballI)?)
-  fix \<iota> and ls :: "label list"
-  assume
-    "\<iota> \<in> Inf_F"
-    "length ls = length (prems_of \<iota>)"
-  then show "\<exists>l. Infer (zip (prems_of \<iota>) ls) (concl_of \<iota>, l) \<in> Inf_FL"
-    unfolding Inf_FL_def Infer_FL_of_def by force
-next
-  fix \<iota>
-  assume "\<iota> \<in> Inf_FL"
-  then show "Infer (map fst (prems_of \<iota>)) (fst (concl_of \<iota>)) \<in> Inf_F"
-    unfolding Inf_FL_def Infer_FL_of_def by auto
-next
   show "equivp (\<doteq>)"
     unfolding equivp_def by (meson generalizes_refl generalizes_trans)
 next
@@ -393,10 +364,10 @@ next
     unfolding wfp_on_UNIV by (metis wf_strictly_generalizes)
 next
   show "po_on (\<sqsubset>l) UNIV"
-    unfolding po_on_def irreflp_on_def transp_on_def using irrefl_Prec_l trans_Prec_l by blast
+    unfolding po_on_def irreflp_on_def transp_on_def using irrefl_L_Prec trans_L_Prec by blast
 next
   show "wfp_on (\<sqsubset>l) UNIV"
-    unfolding wfp_on_UNIV by (rule wf_Prec_l)
+    unfolding wfp_on_UNIV by (rule wf_L_Prec)
 next
   fix C1 D1 C2 D2
   assume
@@ -404,13 +375,13 @@ next
     "C2 \<doteq> D2"
     "C1 \<prec>\<cdot> C2"
   then show "D1 \<prec>\<cdot> D2"
-    by (smt antisym size_mset_mono size_subst strictly_generalizes_def generalizes_def generalizes_trans)
+    by (smt antisym size_mset_mono size_subst strictly_generalizes_def generalizes_def
+        generalizes_trans)
 next
   fix N C1 C2
   assume "C1 \<doteq> C2"
   then show "\<G>_F C1 \<subseteq> \<G>_F C2"
-    unfolding generalizes_def \<G>_F_def
-    by clarsimp (metis is_ground_comp_subst subst_cls_comp_subst)
+    unfolding generalizes_def \<G>_F_def by clarsimp (metis is_ground_comp_subst subst_cls_comp_subst)
 next
   fix N C2 C1
   assume "C2 \<prec>\<cdot> C1"
@@ -418,68 +389,40 @@ next
     unfolding strictly_generalizes_def generalizes_def \<G>_F_def
     by clarsimp (metis is_ground_comp_subst subst_cls_comp_subst)
 next
-  fix \<iota>
-  assume "\<iota> \<in> Inf_F"
-  then show "prems_of \<iota> \<noteq> []"
-    by (simp add: Inf_F_have_prems)
-next
-  fix l
-  assume "l \<noteq> Old"
-  then show "Prec_l Old l"
-    by simp
-next
-  show "\<exists>l. Prec_l Old l"
-    using Prec_l.simps(1) by blast
-next
-  fix \<iota>
-  assume "\<iota> \<in> Inf_FL"
-  then show "snd (concl_of \<iota>) \<noteq> Old"
-    unfolding Inf_FL_def Infer_FL_of_def by auto
-qed
+  show "\<exists>l. L_Prec Old l"
+    using L_Prec.simps(1) by blast
+qed (auto simp: FL_Inf_def FL_Infer_of_def F_Inf_have_prems)
 
-notation GC.Prec_FL (infix "\<sqsubset>" 50)
-notation GC.entails_\<G>_L_Q (infix "\<TTurnstile>\<G>Le" 50)
-notation GC.derive (infix "\<rhd>RedFL" 50)
-notation GC.step (infix "\<Longrightarrow>GC" 50)
+notation FL.Prec_FL (infix "\<sqsubset>" 50)
+notation FL.entails_\<G>_L_Q (infix "\<TTurnstile>\<G>Le" 50)
+notation FL.derive (infix "\<rhd>RedFL" 50)
+notation FL.step (infix "\<Longrightarrow>GC" 50)
 
-lemmas GC_entails_\<G>_L_Q_iff = GC.labeled_entailment_lifting
-
-(* FIXME: Needed? *)
-lemma F_Red_Inf_\<G>_Q_eq:
-  "F.Red_Inf_\<G>_Q N = {\<iota> \<in> Inf_F. \<forall>M. \<G>_Inf M \<iota> \<subseteq> G.Red_Inf M (\<Union> (\<G>_F ` N))}"
-  unfolding F.Red_Inf_\<G>_Q_def F.Red_Inf_\<G>_q_def by auto
-
-lemma GC_Red_Inf_Q_eq:
-  "GC.Red_Inf_Q Nl = {\<iota> \<in> Inf_FL. \<forall>M. the (GC.\<G>_Inf_L_q M \<iota>) \<subseteq> G.Red_Inf M (\<Union> (\<G>_F ` fst ` Nl))}"
-  unfolding GC.Red_Inf_Q_def GC.Red_Inf_\<G>_q_def by auto
-
-lemma GC_Red_F_Q_eq:
-  "GC.Red_F_Q N =
+lemma FL_Red_F_Q_eq:
+  "FL.Red_F_Q N =
    {C. \<forall>D \<in> \<G>_F (fst C).
       D \<in> G.Red_F (\<Union> (\<G>_F ` fst ` N)) \<or> (\<exists>E \<in> N. E \<sqsubset> C \<and> D \<in> \<G>_F (fst E))}"
-  unfolding GC.Red_F_Q_def GC.Red_F_\<G>_q_g_def by auto
+  unfolding FL.Red_F_Q_def FL.Red_F_\<G>_q_g_def by auto
 
-lemma mem_GC_Red_F_Q_because_G_Red_F:
-  "(\<forall>D \<in> \<G>_F (fst Cl). D \<in> G.Red_F (\<Union> (\<G>_F ` fst ` N))) \<Longrightarrow> Cl \<in> GC.Red_F_Q N"
-  unfolding GC_Red_F_Q_eq by auto
+lemma mem_FL_Red_F_Q_because_G_Red_F:
+  "(\<forall>D \<in> \<G>_F (fst Cl). D \<in> G.Red_F (\<Union> (\<G>_F ` fst ` N))) \<Longrightarrow> Cl \<in> FL.Red_F_Q N"
+  unfolding FL_Red_F_Q_eq by auto
 
-lemma mem_GC_Red_F_Q_because_Prec_FL:
-  "(\<forall>D \<in> \<G>_F (fst Cl). \<exists>El \<in> N. El \<sqsubset> Cl \<and> D \<in> \<G>_F (fst El)) \<Longrightarrow> Cl \<in> GC.Red_F_Q N"
-  unfolding GC_Red_F_Q_eq by auto
+lemma mem_FL_Red_F_Q_because_Prec_FL:
+  "(\<forall>D \<in> \<G>_F (fst Cl). \<exists>El \<in> N. El \<sqsubset> Cl \<and> D \<in> \<G>_F (fst El)) \<Longrightarrow> Cl \<in> FL.Red_F_Q N"
+  unfolding FL_Red_F_Q_eq by auto
 
-interpretation GC: refute_compact_consequence_relation GC.Bot_FL "(\<TTurnstile>\<G>Le)"
+interpretation FL: refute_compact_consequence_relation FL.Bot_FL "(\<TTurnstile>\<G>Le)"
 proof
   fix CCl
-  assume unsat: "CCl \<TTurnstile>\<G>Le GC.Bot_FL"
+  assume unsat: "CCl \<TTurnstile>\<G>Le FL.Bot_FL"
 
   let ?bot = "({#}, undefined)"
 
   have "CCl \<TTurnstile>\<G>Le {?bot}"
-    using unsat
-    apply (subst (asm) GC.entail_set_all_formulas)
-    by auto
+    using unsat by (metis (lifting) FL.entail_set_all_formulas UNIV_I insertI1 mem_Sigma_iff)
   then have "\<not> satisfiable (\<Union>CL \<in> CCl. \<G>_F (fst CL))"
-    unfolding GC_entails_\<G>_L_Q_iff F_entails_\<G>_Q_iff by auto
+    unfolding FL.labeled_entailment_lifting F_entails_\<G>_Q_iff by auto
   then obtain DD where
     d_sub: "DD \<subseteq> (\<Union>Cl \<in> CCl. \<G>_F (fst Cl))" and
     d_fin: "finite DD" and
@@ -491,26 +434,21 @@ proof
 
   have ex_in_cl: "\<exists>Cl. Cl \<in> CCl \<and> D \<in> \<G>_F (fst Cl)" if "D \<in> DD" for D
     using that d_sub by blast
-  then have "DD \<subseteq> (\<Union>Cl \<in> CCl'. \<G>_F (fst Cl))"
-    using ex_in_cl unfolding CCl'_def
-    apply auto
-    by (metis (no_types, lifting) eq_fst_iff ex_in_cl someI_ex)
+  then have d_sub': "DD \<subseteq> (\<Union>Cl \<in> CCl'. \<G>_F (fst Cl))"
+    using ex_in_cl unfolding CCl'_def by clarsimp (metis (lifting) eq_fst_iff ex_in_cl someI_ex)
   have "CCl' \<subseteq> CCl"
-    unfolding CCl'_def
-    apply clarsimp
-    using someI_ex[OF ex_in_cl]
-    by blast
+    unfolding CCl'_def using someI_ex[OF ex_in_cl] by blast
   moreover have "finite CCl'"
     unfolding CCl'_def using d_fin by simp
-  moreover have "CCl' \<TTurnstile>\<G>Le GC.Bot_FL"
-    unfolding CCl'_def using d_unsat ex_in_cl
-    by (metis (no_types, lifting) CCl'_def GC.entails_\<G>_L_Q_def \<open>DD \<subseteq> (\<Union>Cl\<in>CCl'. \<G>_F (fst Cl))\<close> subsetD true_clss_def)
-  ultimately show "\<exists>CCl' \<subseteq> CCl. finite CCl' \<and> CCl' \<TTurnstile>\<G>Le GC.Bot_FL"
+  moreover have "CCl' \<TTurnstile>\<G>Le FL.Bot_FL"
+    unfolding CCl'_def using d_unsat ex_in_cl d_sub' CCl'_def
+    by (metis (no_types, lifting) FL.entails_\<G>_L_Q_def subsetD true_clss_def)
+  ultimately show "\<exists>CCl' \<subseteq> CCl. finite CCl' \<and> CCl' \<TTurnstile>\<G>Le FL.Bot_FL"
     by blast
 qed
 
-interpretation GC: refute_compact_calculus_with_red_crit GC.Bot_FL Inf_FL "(\<TTurnstile>\<G>Le)" GC.Red_Inf_Q
-  GC.Red_F_Q
+interpretation FL: refute_compact_calculus_with_red_crit FL.Bot_FL FL_Inf "(\<TTurnstile>\<G>Le)" FL.Red_Inf_Q
+  FL.Red_F_Q
   ..
 
 
@@ -572,20 +510,46 @@ lemma lclss_Liminf_commute:
   apply (meson Pair_inject inj_onI)+
   done
 
-definition RP_infer_of :: "'a clause inference \<Rightarrow> 'a inference_RP" where
-  "RP_infer_of \<iota> = Infer_RP (mset (side_prems_of \<iota>)) (main_prem_of \<iota>) (concl_of \<iota>)"
+lemma GC_tautology_step:
+  assumes tauto: "Neg A \<in># C" "Pos A \<in># C"
+  shows "lclss_of_state (N \<union> {C}, P, Q) \<Longrightarrow>GC lclss_of_state (N, P, Q)"
+proof -
+  have c\<theta>_red:
+    "C\<theta> \<in> G.Red_F (\<Union>D \<in> N'. \<G>_F (fst D))" if in_g: "C\<theta> \<in> \<G>_F C"
+    for N' :: "('a clause \<times> label) set" and C\<theta>
+  proof -
+    obtain \<theta> where
+      "C\<theta> = C \<cdot> \<theta>"
+       using in_g unfolding \<G>_F_def by blast
+    then have compl_lits:
+      "Neg (A \<cdot>a \<theta>) \<in># C\<theta>"
+      "Pos (A \<cdot>a \<theta>) \<in># C\<theta>"
+      using tauto Neg_Melem_subst_atm_subst_cls Pos_Melem_subst_atm_subst_cls by auto
+    then have "{} \<TTurnstile>e {C\<theta>}"
+      unfolding true_clss_def true_cls_def true_lit_def if_distrib_fun
+      by (metis literal.disc literal.sel singletonD)
+    then show ?thesis
+      unfolding G.Red_F_def by auto
+  qed
 
-lemma gc_subsumption_step:
+  show ?thesis
+    apply (rule FL.step.process[of _ "lclss_of_state (N, P, Q)" "{(C, New)}" _ "{}"])
+    apply (auto simp: lclss_of_state_def FL.active_subset_def)
+    apply (rule mem_FL_Red_F_Q_because_G_Red_F)
+    using c\<theta>_red[of _ "lclss_of_state (N, P, Q)"] unfolding lclss_of_state_def by auto
+qed
+
+lemma GC_subsumption_step:
   assumes
     d_in: "Dl \<in> N" and
     d_sub_c: "strictly_subsumes (fst Dl) (fst Cl) \<or> subsumes (fst Dl) (fst Cl) \<and> snd Dl \<sqsubset>l snd Cl"
   shows "N \<union> {Cl} \<Longrightarrow>GC N"
 proof -
-  have d_sub'_c: "Cl \<in> GC.Red_F_Q {Dl} \<or> Dl \<sqsubset> Cl"
+  have d_sub'_c: "Cl \<in> FL.Red_F_Q {Dl} \<or> Dl \<sqsubset> Cl"
   proof (cases "size (fst Dl) = size (fst Cl)")
     case True
     then have "Dl \<sqsubset> Cl"
-      apply (unfold GC.Prec_FL_def Prover_Architecture_Basis.Prec_FL_def)
+      apply (unfold FL.Prec_FL_def Prover_Architecture_Basis.Prec_FL_def)
       apply (unfold generalizes_def strictly_generalizes_def)
       using d_sub_c
       apply (unfold strictly_subsumes_def subsumes_def)
@@ -597,9 +561,10 @@ proof -
     then have d_ssub_c: "strictly_subsumes (fst Dl) (fst Cl)"
       using d_sub_c
       apply (unfold strictly_subsumes_def subsumes_def)
-      by (metis size_subst strict_subset_subst_strictly_subsumes strictly_subsumes_antisym subset_mset.antisym_conv2)
-    have "Cl \<in> GC.Red_F_Q {Dl}"
-      apply (rule mem_GC_Red_F_Q_because_G_Red_F)
+      by (metis size_subst strict_subset_subst_strictly_subsumes strictly_subsumes_antisym
+          subset_mset.antisym_conv2)
+    have "Cl \<in> FL.Red_F_Q {Dl}"
+      apply (rule mem_FL_Red_F_Q_because_G_Red_F)
       apply (unfold G.Red_F_def)
       apply clarsimp
       using d_ssub_c
@@ -618,23 +583,23 @@ proof -
       by (rule disjI1)
   qed
   show ?thesis
-    apply (rule GC.step.process[of _ N "{Cl}" _ "{}"])
+    apply (rule FL.step.process[of _ N "{Cl}" _ "{}"])
        apply auto
-    using d_sub'_c unfolding GC_Red_F_Q_eq
+    using d_sub'_c unfolding FL_Red_F_Q_eq
      apply auto
     apply (metis (no_types, lifting) G.Red_F_of_subset SUP_upper d_in subset_iff)
-      apply (smt GC.Prec_FL_def GC.equiv_F_grounding GC.prec_F_grounding UNIV_witness d_in in_mono)
-    by (simp add: GC.active_subset_def)+
+      apply (smt FL.Prec_FL_def FL.equiv_F_grounding FL.prec_F_grounding UNIV_witness d_in in_mono)
+    by (simp add: FL.active_subset_def)+
 qed
 
-lemma gc_reduction_step:
+lemma GC_reduction_step:
   assumes
-    passiv: "snd Dl \<noteq> Old" and
+    young: "snd Dl \<noteq> Old" and
     d_sub_c: "fst Dl \<subset># fst Cl"
   shows "N \<union> {Cl} \<Longrightarrow>GC N \<union> {Dl}"
-proof (rule GC.step.process[of _ N "{Cl}" _ "{Dl}"])
-  have "Cl \<in> GC.Red_F_Q {Dl}"
-    apply (rule mem_GC_Red_F_Q_because_G_Red_F)
+proof (rule FL.step.process[of _ N "{Cl}" _ "{Dl}"])
+  have "Cl \<in> FL.Red_F_Q {Dl}"
+    apply (rule mem_FL_Red_F_Q_because_G_Red_F)
     apply (unfold G.Red_F_def)
     apply clarsimp
     unfolding \<G>_F_def
@@ -646,44 +611,37 @@ proof (rule GC.step.process[of _ N "{Cl}" _ "{Dl}"])
      apply fast
     using subst_subset_mono[OF d_sub_c]
     by (simp add: subset_imp_less_mset)
-  then show "{Cl} \<subseteq> GC.Red_F_Q (N \<union> {Dl})"
-    using GC.Red_F_of_subset by blast
-qed (auto simp: GC.active_subset_def passiv)
+  then show "{Cl} \<subseteq> FL.Red_F_Q (N \<union> {Dl})"
+    using FL.Red_F_of_subset by blast
+qed (auto simp: FL.active_subset_def young)
 
-lemma gc_processing_step: "N \<union> {(C, New)} \<Longrightarrow>GC N \<union> {(C, Processed)}"
-proof (rule GC.step.process[of _ N "{(C, New)}" _ "{(C, Processed)}"])
-  have "(C, New) \<in> GC.Red_F_Q {(C, Processed)}"
-    apply (rule mem_GC_Red_F_Q_because_Prec_FL)
-    unfolding GC.Prec_FL_def
-    apply auto
-    by (simp add: generalizes_refl)
-  then show "{(C, New)} \<subseteq> GC.Red_F_Q (N \<union> {(C, Processed)})"
-    using GC.Red_F_of_subset by blast
-qed (auto simp: GC.active_subset_def)
+lemma GC_processing_step: "N \<union> {(C, New)} \<Longrightarrow>GC N \<union> {(C, Processed)}"
+proof (rule FL.step.process[of _ N "{(C, New)}" _ "{(C, Processed)}"])
+  have "(C, New) \<in> FL.Red_F_Q {(C, Processed)}"
+    by (rule mem_FL_Red_F_Q_because_Prec_FL) (simp add: FL.Prec_FL_def generalizes_refl)
+  then show "{(C, New)} \<subseteq> FL.Red_F_Q (N \<union> {(C, Processed)})"
+    using FL.Red_F_of_subset by blast
+qed (auto simp: FL.active_subset_def)
 
-lemma RP_inferences_between_eq_F_Inf_from2:
-  "concl_of_RP ` inference_system.inferences_between (ord_FO_\<Gamma> S) N C =
+lemma old_inferences_between_eq_new_inferences_between:
+  "old_concl_of ` inference_system.inferences_between (ord_FO_\<Gamma> S) N C =
    concl_of ` F.Inf_from2 N {C}" (is "?rp = ?f")
 proof (intro set_eqI iffI)
   fix E
-  assume e_in: "E \<in> concl_of_RP ` inference_system.inferences_between (ord_FO_\<Gamma> S) N C"
+  assume e_in: "E \<in> old_concl_of ` inference_system.inferences_between (ord_FO_\<Gamma> S) N C"
 
   obtain CAs DA AAs As \<sigma> where
     e_res: "ord_resolve_rename S CAs DA AAs As \<sigma> E" and
     cd_sub: "set CAs \<union> {DA} \<subseteq> N \<union> {C}" and
     c_in: "C \<in> set CAs \<union> {DA}"
-    using e_in
-    unfolding inference_system.inferences_between_def infer_from_def ord_FO_\<Gamma>_def
-    apply auto
-    done
+    using e_in unfolding inference_system.inferences_between_def infer_from_def ord_FO_\<Gamma>_def by auto
 
   show "E \<in> concl_of ` F.Inf_from2 N {C}"
-    unfolding F.Inf_from2_alt F.Inf_from_def Inf_F_def inference_system.Inf_from2_alt
+    unfolding F.Inf_from2_alt F.Inf_from_def F_Inf_def inference_system.Inf_from2_alt
       inference_system.Inf_from_def
-    apply (auto simp: image_def Bex_def)
+    apply (auto simp: image_def)
     apply (rule_tac x = "Infer (CAs @ [DA]) E" in exI)
-    apply auto
-    using e_res cd_sub c_in apply auto done
+    using e_res cd_sub c_in by auto
 next
   fix E
   assume e_in: "E \<in> concl_of ` F.Inf_from2 N {C}"
@@ -692,87 +650,51 @@ next
     e_res: "ord_resolve_rename S CAs DA AAs As \<sigma> E" and
     cd_sub: "set CAs \<union> {DA} \<subseteq> N \<union> {C}" and
     c_in: "C \<in> set CAs \<union> {DA}"
-    using e_in
-    unfolding F.Inf_from2_alt F.Inf_from_def Inf_F_def inference_system.Inf_from2_alt
+    using e_in unfolding F.Inf_from2_alt F.Inf_from_def F_Inf_def inference_system.Inf_from2_alt
       inference_system.Inf_from_def
-    apply (auto simp: image_def Bex_def)
-    done
+    by (auto simp: image_def Bex_def)
 
-  show "E \<in> concl_of_RP ` inference_system.inferences_between (ord_FO_\<Gamma> S) N C"
+  show "E \<in> old_concl_of ` inference_system.inferences_between (ord_FO_\<Gamma> S) N C"
     unfolding inference_system.inferences_between_def infer_from_def ord_FO_\<Gamma>_def
     using e_res cd_sub c_in
     apply (clarsimp simp: image_def Bex_def)
-    apply (rule_tac x = "Infer_RP (mset CAs) DA E" in exI)
-    apply auto
-    done
+    apply (rule_tac x = "old_Infer (mset CAs) DA E" in exI)
+    by auto
 qed
 
-lemma gc_inference_step:
+lemma GC_inference_step:
   assumes
-    l_ne: "l \<noteq> Old" and
-    m_passiv: "GC.active_subset M = {}" and
-    m_sup: "fst ` M \<supseteq> concl_of_RP ` inference_system.inferences_between (ord_FO_\<Gamma> S)
-      (fst ` GC.active_subset N) C"
+    young: "l \<noteq> Old" and
+    no_active: "FL.active_subset M = {}" and
+    m_sup: "fst ` M \<supseteq> old_concl_of ` inference_system.inferences_between (ord_FO_\<Gamma> S)
+      (fst ` FL.active_subset N) C"
   shows "N \<union> {(C, l)} \<Longrightarrow>GC N \<union> {(C, Old)} \<union> M"
-proof (rule GC.step.infer[of _ N C l _ M])
-  have m_sup': "fst ` M \<supseteq> concl_of ` F.Inf_from2 (fst ` GC.active_subset N) {C}"
-    using m_sup unfolding RP_inferences_between_eq_F_Inf_from2 .
+proof (rule FL.step.infer[of _ N C l _ M])
+  have m_sup': "fst ` M \<supseteq> concl_of ` F.Inf_from2 (fst ` FL.active_subset N) {C}"
+    using m_sup unfolding old_inferences_between_eq_new_inferences_between .
 
-  show "F.Inf_from2 (fst ` GC.active_subset N) {C} \<subseteq> F.Red_Inf_Q (fst ` (N \<union> {(C, Old)} \<union> M))"
+  show "F.Inf_from2 (fst ` FL.active_subset N) {C} \<subseteq> F.Red_Inf_Q (fst ` (N \<union> {(C, Old)} \<union> M))"
   proof
     fix \<iota>
-    assume \<iota>_in_if2: "\<iota> \<in> F.Inf_from2 (fst ` GC.active_subset N) {C}"
+    assume \<iota>_in_if2: "\<iota> \<in> F.Inf_from2 (fst ` FL.active_subset N) {C}"
 
-    have \<iota>_in: "\<iota> \<in> Inf_F"
+    have \<iota>_in: "\<iota> \<in> F_Inf"
       using \<iota>_in_if2 unfolding F.Inf_from2_def F.Inf_from_def by auto
 
     have "concl_of \<iota> \<in> fst ` M"
-      using m_sup'
-      apply (auto simp: image_def Collect_mono_iff F.Inf_from2_alt)
-      using \<iota>_in_if2 m_sup' by auto
+      using m_sup' \<iota>_in_if2 m_sup' by (auto simp: image_def Collect_mono_iff F.Inf_from2_alt)
     then have "concl_of \<iota> \<in> fst ` (N \<union> {(C, Old)} \<union> M)"
       by auto
     then show "\<iota> \<in> F.Red_Inf_\<G>_Q (fst ` (N \<union> {(C, Old)} \<union> M))"
       by (rule F.Red_Inf_of_Inf_to_N[OF \<iota>_in])
   qed
-qed (use l_ne m_passiv in auto)
+qed (use young no_active in auto)
 
-lemma step_RP_imp_step_GC: "St \<leadsto> St' \<Longrightarrow> lclss_of_state St \<Longrightarrow>GC lclss_of_state St'"
+lemma RP_step_imp_GC_step: "St \<leadsto> St' \<Longrightarrow> lclss_of_state St \<Longrightarrow>GC lclss_of_state St'"
 proof (induction rule: RP.induct)
   case (tautology_deletion A C N P Q)
-  note tauto = this
-
-  have c\<theta>_red:
-    "C\<theta> \<in> G.Red_F (\<Union>D \<in> N'. \<G>_F (fst D))" if in_g: "C\<theta> \<in> \<G>_F C"
-    for N' :: "('a clause \<times> label) set" and C\<theta>
-  proof -
-    obtain \<theta> where
-      "C\<theta> = C \<cdot> \<theta>"
-       using in_g unfolding \<G>_F_def by blast
-    then have compl_lits:
-      "Neg (A \<cdot>a \<theta>) \<in># C\<theta>"
-      "Pos (A \<cdot>a \<theta>) \<in># C\<theta>"
-      using tauto Neg_Melem_subst_atm_subst_cls Pos_Melem_subst_atm_subst_cls by auto
-    then have "{} \<TTurnstile>e {C\<theta>}"
-      unfolding true_clss_def true_cls_def true_lit_def if_distrib_fun
-      by (metis (full_types) literal.disc(1,2) literal.sel(1,2) singletonD)
-    then show ?thesis
-      unfolding G.Red_F_def
-      apply clarsimp
-      apply (rule exI[of _ "{}"])
-      apply clarsimp
-      done
-  qed
-
-  show ?case
-    apply (rule GC.step.process[of _ "lclss_of_state (N, P, Q)" "{(C, New)}" _ "{}"])
-    apply (auto simp: lclss_of_state_def GC.active_subset_def)
-    apply (rule mem_GC_Red_F_Q_because_G_Red_F)
-    apply (unfold image_Un image_comp[of fst])
-    apply (unfold image_Un[symmetric])
-    apply simp
-    using c\<theta>_red[of _ "lclss_of_state (N, P, Q)"] unfolding lclss_of_state_def
-    by auto
+  then show ?case
+    by (rule GC_tautology_step)
 next
   case (forward_subsumption D P Q C N)
   note d_in = this(1) and d_sub_c = this(2)
@@ -780,119 +702,117 @@ next
   proof (cases "D \<in> P")
     case True
     then show ?thesis
-      using gc_subsumption_step[of "(D, Processed)" "lclss_of_state (N, P, Q)" "(C, New)"] d_sub_c
+      using GC_subsumption_step[of "(D, Processed)" "lclss_of_state (N, P, Q)" "(C, New)"] d_sub_c
       by auto
   next
     case False
     then have "D \<in> Q"
       using d_in by simp
     then show ?thesis
-      using gc_subsumption_step[of "(D, Old)" "lclss_of_state (N, P, Q)" "(C, New)"] d_sub_c by auto
+      using GC_subsumption_step[of "(D, Old)" "lclss_of_state (N, P, Q)" "(C, New)"] d_sub_c by auto
   qed
 next
   case (backward_subsumption_P D N C P Q)
   note d_in = this(1) and d_ssub_c = this(2)
   then show ?case
-    using gc_subsumption_step[of "(D, New)" "lclss_of_state (N, P, Q)" "(C, Processed)"] d_ssub_c
+    using GC_subsumption_step[of "(D, New)" "lclss_of_state (N, P, Q)" "(C, Processed)"] d_ssub_c
     by auto
 next
   case (backward_subsumption_Q D N C P Q)
   note d_in = this(1) and d_ssub_c = this(2)
   then show ?case
-    using gc_subsumption_step[of "(D, New)" "lclss_of_state (N, P, Q)" "(C, Old)"] d_ssub_c by auto
+    using GC_subsumption_step[of "(D, New)" "lclss_of_state (N, P, Q)" "(C, Old)"] d_ssub_c by auto
 next
   case (forward_reduction D L' P Q L \<sigma> C N)
   show ?case
-    using gc_reduction_step[of "(C, New)" "(C + {#L#}, New)" "lclss_of_state (N, P, Q)"] by auto
+    using GC_reduction_step[of "(C, New)" "(C + {#L#}, New)" "lclss_of_state (N, P, Q)"] by auto
 next
   case (backward_reduction_P D L' N L \<sigma> C P Q)
   show ?case
-    using gc_reduction_step[of "(C, Processed)" "(C + {#L#}, Processed)" "lclss_of_state (N, P, Q)"]
+    using GC_reduction_step[of "(C, Processed)" "(C + {#L#}, Processed)" "lclss_of_state (N, P, Q)"]
     by auto
 next
   case (backward_reduction_Q D L' N L \<sigma> C P Q)
   show ?case
-    using gc_reduction_step[of "(C, Processed)" "(C + {#L#}, Old)" "lclss_of_state (N, P, Q)"]
+    using GC_reduction_step[of "(C, Processed)" "(C + {#L#}, Old)" "lclss_of_state (N, P, Q)"]
     by auto
 next
   case (clause_processing N C P Q)
   show ?case
-    using gc_processing_step[of "lclss_of_state (N, P, Q)" C] by auto
+    using GC_processing_step[of "lclss_of_state (N, P, Q)" C] by auto
 next
   case (inference_computation N Q C P)
   note n = this(1)
   show ?case
-    apply (auto simp: GC.active_subset_def)
-    apply (rule gc_inference_step[of Processed "lclss_of_state (N, {}, {})" "lclss_of_state ({}, P, Q)" C,
-        simplified])
-    unfolding n apply (auto simp: GC.active_subset_def)
+    apply (auto simp: FL.active_subset_def)
+    apply (rule GC_inference_step[of Processed "lclss_of_state (N, {}, {})"
+          "lclss_of_state ({}, P, Q)" C, simplified])
+    unfolding n apply (auto simp: FL.active_subset_def)
     unfolding inference_system.inferences_between_def image_def mem_Collect_eq lclss_of_state_def
       infer_from_def
-    apply auto
-    done
+    by auto
 qed
 
-lemma derivation_RP_imp_derivation_GC: "chain (\<leadsto>) Sts \<Longrightarrow> chain (\<Longrightarrow>GC) (lmap lclss_of_state Sts)"
-  using chain_lmap step_RP_imp_step_GC by blast
+lemma RP_derivation_imp_GC_derivation: "chain (\<leadsto>) Sts \<Longrightarrow> chain (\<Longrightarrow>GC) (lmap lclss_of_state Sts)"
+  using chain_lmap RP_step_imp_GC_step by blast
 
-lemma step_RP_imp_step: "St \<leadsto> St' \<Longrightarrow> lclss_of_state St \<rhd>RedFL lclss_of_state St'"
-  by (rule GC.one_step_equiv) (rule step_RP_imp_step_GC)
+lemma RP_step_imp_RedFL_step: "St \<leadsto> St' \<Longrightarrow> lclss_of_state St \<rhd>RedFL lclss_of_state St'"
+  by (rule FL.one_step_equiv) (rule RP_step_imp_GC_step)
 
-lemma derivation_RP_imp_derivation_RedFL: "chain (\<leadsto>) Sts \<Longrightarrow> chain (\<rhd>RedFL) (lmap lclss_of_state Sts)"
-  using chain_lmap step_RP_imp_step by blast
+lemma RP_derivation_imp_RedFL_derivation:
+  "chain (\<leadsto>) Sts \<Longrightarrow> chain (\<rhd>RedFL) (lmap lclss_of_state Sts)"
+  using chain_lmap RP_step_imp_RedFL_step by blast
 
 theorem RP_sound_new_statement:
   assumes
     deriv: "chain (\<leadsto>) Sts" and
     bot_in: "{#} \<in> clss_of_state (Liminf_state Sts)"
-  shows "grounding_of_state (lhd Sts) \<TTurnstile>e {{#}}"
+  shows "clss_of_state (lhd Sts) \<TTurnstile>\<G>e {{#}}"
 proof -
   have "clss_of_state (Liminf_state Sts) \<TTurnstile>\<G>e {{#}}"
     using F.subset_entailed bot_in by auto
   then have "fst ` Liminf_llist (lmap lclss_of_state Sts) \<TTurnstile>\<G>e {{#}}"
     by (metis image_fst_lclss_of_state lclss_Liminf_commute)
-  then have "Liminf_llist (lmap lclss_of_state Sts) \<TTurnstile>\<G>Le GC.Bot_FL"
-    using GC.labeled_entailment_lifting by simp
-  then have "lhd (lmap lclss_of_state Sts) \<TTurnstile>\<G>Le GC.Bot_FL"
+  then have "Liminf_llist (lmap lclss_of_state Sts) \<TTurnstile>\<G>Le FL.Bot_FL"
+    using FL.labeled_entailment_lifting by simp
+  then have "lhd (lmap lclss_of_state Sts) \<TTurnstile>\<G>Le FL.Bot_FL"
     apply -
-    apply (subst (asm) GC.unsat_limit_iff)
-    using deriv derivation_RP_imp_derivation_RedFL apply auto[1]
-    defer
-    apply blast
-    by (smt F_entails_\<G>_Q_iff GC_entails_\<G>_L_Q_iff RP_model chain_lmap deriv grounding_of_clss_def
+    apply (subst (asm) FL.unsat_limit_iff)
+    using deriv RP_derivation_imp_RedFL_derivation
+      apply simp
+    apply (smt F_entails_\<G>_Q_iff FL.labeled_entailment_lifting RP_model chain_lmap deriv \<G>_Fs_def
         image_fst_lclss_of_state)
-  then have "lclss_of_state (lhd Sts) \<TTurnstile>\<G>Le GC.Bot_FL"
+    by blast
+  then have "lclss_of_state (lhd Sts) \<TTurnstile>\<G>Le FL.Bot_FL"
     using chain_not_lnull deriv by fastforce
-  then have "clss_of_state (lhd Sts) \<TTurnstile>\<G>e {{#}}"
-    unfolding GC.entails_\<G>_L_Q_def F.entails_\<G>_Q_def lclss_of_state_def by auto
   then show ?thesis
-    using F_entails_\<G>_Q_iff grounding_of_clss_def by auto
+    unfolding FL.entails_\<G>_L_Q_def F.entails_\<G>_Q_def lclss_of_state_def by auto
 qed
 
 theorem RP_saturated_if_fair_new_statement:
   assumes
     deriv: "chain (\<leadsto>) Sts" and
-    init: "GC.active_subset (lnth (lmap lclss_of_state Sts) 0) = {}" and
-    final: "GC.passive_subset (Liminf_llist (lmap lclss_of_state Sts)) = {}"
-  shows "GC.saturated (Liminf_llist (lmap lclss_of_state Sts))"
+    init: "FL.active_subset (lnth (lmap lclss_of_state Sts) 0) = {}" and
+    final: "FL.passive_subset (Liminf_llist (lmap lclss_of_state Sts)) = {}"
+  shows "FL.saturated (Liminf_llist (lmap lclss_of_state Sts))"
 proof -
   have gc_deriv: "chain (\<Longrightarrow>GC) (lmap lclss_of_state Sts)"
-    by (rule derivation_RP_imp_derivation_GC[OF deriv])
+    by (rule RP_derivation_imp_GC_derivation[OF deriv])
   show ?thesis
-    by (rule GC.fair_implies_Liminf_saturated[OF GC.gc_to_red[OF gc_deriv]
-          GC.gc_fair[OF gc_deriv init final]])
+    by (rule FL.fair_implies_Liminf_saturated[OF FL.gc_to_red[OF gc_deriv]
+          FL.gc_fair[OF gc_deriv init final]])
 qed
 
 corollary RP_complete_if_fair_new_statement:
   assumes
     deriv: "chain (\<leadsto>) Sts" and
-    init: "GC.active_subset (lnth (lmap lclss_of_state Sts) 0) = {}" and
-    final: "GC.passive_subset (Liminf_llist (lmap lclss_of_state Sts)) = {}" and
+    init: "FL.active_subset (lnth (lmap lclss_of_state Sts) 0) = {}" and
+    final: "FL.passive_subset (Liminf_llist (lmap lclss_of_state Sts)) = {}" and
     unsat: "grounding_of_state (lhd Sts) \<TTurnstile>e {{#}}"
   shows "{#} \<in> Q_of_state (Liminf_state Sts)"
 proof -
   have gc_deriv: "chain (\<Longrightarrow>GC) (lmap lclss_of_state Sts)"
-    by (rule derivation_RP_imp_derivation_GC[OF deriv])
+    by (rule RP_derivation_imp_GC_derivation[OF deriv])
   have fst_unsat: "fst ` lnth (lmap lclss_of_state Sts) 0 \<TTurnstile>\<G>e {{#}}"
   proof -
     have len: "llength Sts > 0"
@@ -910,15 +830,14 @@ proof -
       apply auto
       apply (erule_tac x = I in allE)
       apply (erule bexE)
-      unfolding grounding_of_clss_def
+      unfolding \<G>_Fs_def
       by (metis UN_E)
   qed
-  have "\<exists>BL \<in> {{#}} \<times> UNIV. BL \<in> Liminf_llist (lmap lclss_of_state Sts)"
-    using GC.gc_complete_Liminf[OF gc_deriv init final _ fst_unsat] by blast
   then show ?thesis
+    using FL.gc_complete_Liminf[OF gc_deriv init final _ fst_unsat]
     unfolding lclss_Liminf_commute
     unfolding lclss_of_state_def
-    using final[unfolded GC.passive_subset_def]
+    using final[unfolded FL.passive_subset_def]
     apply auto
     using Liminf_state_def lclss_Liminf_commute apply fastforce
     using Liminf_state_def lclss_Liminf_commute by fastforce
@@ -927,34 +846,30 @@ qed
 
 subsection \<open>Alternative Derivation of Previous RP Results\<close>
 
-lemma fair_RP_imp_fair:
+lemma old_fair_imp_new_fair:
   assumes
     nnul: "\<not> lnull Sts" and
     fair: "fair_state_seq Sts" and
     empty_Q0: "Q_of_state (lhd Sts) = {}"
   shows
-    "GC.active_subset (lnth (lmap lclss_of_state Sts) 0) = {}" and
-    "GC.passive_subset (Liminf_llist (lmap lclss_of_state Sts)) = {}"
+    "FL.active_subset (lnth (lmap lclss_of_state Sts) 0) = {}"
+    "FL.passive_subset (Liminf_llist (lmap lclss_of_state Sts)) = {}"
 proof -
-  show "GC.active_subset (lnth (lmap lclss_of_state Sts) 0) = {}"
-    using empty_Q0 unfolding GC.active_subset_def
-    using nnul
-    apply (cases Sts)
-    apply auto
-    done
+  show "FL.active_subset (lnth (lmap lclss_of_state Sts) 0) = {}"
+    using nnul empty_Q0 unfolding FL.active_subset_def by (cases Sts) auto
 next
-  show "GC.passive_subset (Liminf_llist (lmap lclss_of_state Sts)) = {}"
-    using fair unfolding fair_state_seq_def GC.passive_subset_def
+  show "FL.passive_subset (Liminf_llist (lmap lclss_of_state Sts)) = {}"
+    using fair unfolding fair_state_seq_def FL.passive_subset_def
     apply auto
     unfolding lclss_Liminf_commute
     by (metis (no_types, lifting) Liminf_state_def N_of_state_Liminf P_of_state_Liminf empty_iff
         label.exhaust mem_lclss_of_state(1) mem_lclss_of_state(2))
 qed
 
-lemma redundant_infer_RP_alt:
+lemma old_redundant_infer_iff:
   "src.redundant_infer N \<gamma> \<longleftrightarrow>
-   (\<exists>DD. DD \<subseteq> N \<and> DD \<union> set_mset (side_prems_of_RP \<gamma>) \<TTurnstile>e {concl_of_RP \<gamma>}
-      \<and> (\<forall>D \<in> DD. D < main_prem_of_RP \<gamma>))"
+   (\<exists>DD. DD \<subseteq> N \<and> DD \<union> set_mset (old_side_prems_of \<gamma>) \<TTurnstile>e {old_concl_of \<gamma>}
+      \<and> (\<forall>D \<in> DD. D < old_main_prem_of \<gamma>))"
   (is "?lhs \<longleftrightarrow> ?rhs")
 proof
   assume ?lhs
@@ -964,37 +879,33 @@ next
   assume ?rhs
   then obtain DD0 where
     "DD0 \<subseteq> N" and
-    "DD0 \<union> set_mset (side_prems_of_RP \<gamma>) \<TTurnstile>e {concl_of_RP \<gamma>}" and
-    "\<forall>D \<in> DD0. D < main_prem_of_RP \<gamma>"
+    "DD0 \<union> set_mset (old_side_prems_of \<gamma>) \<TTurnstile>e {old_concl_of \<gamma>}" and
+    "\<forall>D \<in> DD0. D < old_main_prem_of \<gamma>"
     by blast
   then obtain DD where
     "finite DD" and
     "DD \<subseteq> N" and
-    "DD \<union> set_mset (side_prems_of_RP \<gamma>) \<TTurnstile>e {concl_of_RP \<gamma>}" and
-    "\<forall>D \<in> DD. D < main_prem_of_RP \<gamma>"
-    using entails_compact_union[of "{concl_of_RP \<gamma>}" DD0 "set_mset (side_prems_of_RP \<gamma>)"] by fast
+    "DD \<union> set_mset (old_side_prems_of \<gamma>) \<TTurnstile>e {old_concl_of \<gamma>}" and
+    "\<forall>D \<in> DD. D < old_main_prem_of \<gamma>"
+    using entails_compact_union[of "{old_concl_of \<gamma>}" DD0 "set_mset (old_side_prems_of \<gamma>)"] by fast
   then show ?lhs
     unfolding src.redundant_infer_def
     apply -
     apply (rule exI[of _ "mset_set DD"])
-    apply auto
-    done
+    by auto
 qed
 
-lemma new_redundant_infer_imp_old_redundant_infer:
-  assumes "G.redundant_infer N \<iota>"
-  shows "src.redundant_infer N (RP_infer_of \<iota>)"
-  using assms
-  unfolding redundant_infer_RP_alt
-  unfolding G.redundant_infer_def RP_infer_of_def
-  by simp
+definition old_infer_of :: "'a clause inference \<Rightarrow> 'a old_inference" where
+  "old_infer_of \<iota> = old_Infer (mset (side_prems_of \<iota>)) (main_prem_of \<iota>) (concl_of \<iota>)"
 
-term src.saturated_upto
+lemma new_redundant_infer_imp_old_redundant_infer:
+  "G.redundant_infer N \<iota> \<Longrightarrow> src.redundant_infer N (old_infer_of \<iota>)"
+  unfolding old_redundant_infer_iff G.redundant_infer_def old_infer_of_def by simp
 
 lemma saturated_imp_saturated_RP:
   assumes
-    satur: "GC.saturated (Liminf_llist (lmap lclss_of_state Sts))" and
-    no_passive: "GC.passive_subset (Liminf_llist (lmap lclss_of_state Sts)) = {}"
+    satur: "FL.saturated (Liminf_llist (lmap lclss_of_state Sts))" and
+    no_passive: "FL.passive_subset (Liminf_llist (lmap lclss_of_state Sts)) = {}"
   shows "src.saturated_upto Sts (grounding_of_state (Liminf_state Sts))"
 proof -
   define Q where
@@ -1004,11 +915,9 @@ proof -
   define G where
     "G = \<Union> (\<G>_F ` Q)"
 
-  note defs = Q_def Ql_def G_def
-
   have limuls_eq: "Liminf_llist (lmap lclss_of_state Sts) = Ql"
     unfolding Ql_def Q_def
-    using no_passive[unfolded GC.passive_subset_def]
+    using no_passive[unfolded FL.passive_subset_def]
     apply simp
   proof - (* sledgehammer *)
     assume a1: "\<forall>a b. (a, b) \<in> Liminf_llist (lmap lclss_of_state Sts) \<longrightarrow> b = Old"
@@ -1043,8 +952,6 @@ proof -
   have gflimuls_eq: "(\<Union>Cl \<in> Ql. \<G>_F (fst Cl)) = G"
     unfolding Ql_def G_def by auto
 
-  note simps = defs[symmetric] limuls_eq clst_eq gflimuls_eq
-
   have "gd.inferences_from Sts G \<subseteq> src.Ri Sts G"
   proof
     fix \<gamma>
@@ -1052,68 +959,59 @@ proof -
 
     obtain \<iota> where
       \<iota>_in_inff: "\<iota> \<in> G.Inf_from Q G" and
-      \<gamma>: "\<gamma> = RP_infer_of \<iota>"
-      using \<gamma>_in_inf unfolding gd.inferences_from_def infer_from_RP_def G.Inf_from_def 
-        RP_infer_of_def
+      \<gamma>: "\<gamma> = old_infer_of \<iota>"
+      using \<gamma>_in_inf unfolding gd.inferences_from_def old_infer_from_def G.Inf_from_def 
+        old_infer_of_def
       apply atomize_elim
       apply auto
-      unfolding gd.ord_\<Gamma>_def Inf_G_def
+      unfolding gd.ord_\<Gamma>_def G_Inf_def
       apply auto
       apply (rule_tac x = "Infer (CAs @ [DA]) E" in exI)
       apply (intro conjI)
       subgoal
-        unfolding defs S_Q_def Liminf_state_def Q_of_state.simps
+        unfolding Q_def S_Q_def Liminf_state_def Q_of_state.simps
         apply auto
       done
-      unfolding simps prems_of_def inference.case set_append
-      apply auto
-      done
+    apply auto
+    done
 
     obtain \<iota>' where
       \<iota>'_in_inff: "\<iota>' \<in> F.Inf_from Q" and
       \<iota>_in_\<iota>': "\<iota> \<in> \<G>_Inf Q \<iota>'"
-      using G_Inf_overapproximates_F_Inf \<iota>_in_inff unfolding defs by blast
+      using G_Inf_overapproximates_F_Inf \<iota>_in_inff unfolding G_def by blast
 
-    have \<iota>'_in_inf: "\<iota>' \<in> Inf_F"
+    have \<iota>'_in_inf: "\<iota>' \<in> F_Inf"
       using F.Inf_from_def \<iota>'_in_inff by blast
 
     let ?olds = "replicate (length (prems_of \<iota>')) Old"
 
     obtain \<iota>'' and l0 where
       \<iota>'': "\<iota>'' = Infer (zip (prems_of \<iota>') ?olds) (concl_of \<iota>', l0)" and
-      \<iota>''_in_inf: "\<iota>'' \<in> Inf_FL"
-      using GC.Inf_F_to_Inf_FL[OF \<iota>'_in_inf, of ?olds, simplified] by blast
+      \<iota>''_in_inf: "\<iota>'' \<in> FL_Inf"
+      using FL.Inf_F_to_Inf_FL[OF \<iota>'_in_inf, of ?olds, simplified] by blast
 
     have "set (prems_of \<iota>'') \<subseteq> Ql"
-      using \<iota>'_in_inff[unfolded F.Inf_from_def, simplified] unfolding \<iota>'' defs by auto
-    then have \<iota>''_in_inff: "\<iota>'' \<in> GC.Inf_from Ql"
-      unfolding GC.Inf_from_def using \<iota>''_in_inf by simp
-    have \<iota>': "\<iota>' = GC.to_F \<iota>''"
-      unfolding \<iota>'' unfolding GC.to_F_def by simp
-
-    have "\<iota> \<in> G.Red_Inf Q G"
-      using \<iota>' \<iota>''_in_inff \<iota>_in_\<iota>'
-        GC.sat_inf_imp_ground_red_fam_inter[OF satur, unfolded simps, simplified]
+      using \<iota>'_in_inff[unfolded F.Inf_from_def, simplified] unfolding \<iota>'' Ql_def by auto
+    then have "\<iota>'' \<in> FL.Inf_from Ql"
+      unfolding FL.Inf_from_def using \<iota>''_in_inf by simp
+    moreover have "\<iota>' = FL.to_F \<iota>''"
+      unfolding \<iota>'' unfolding FL.to_F_def by simp
+    ultimately have "\<iota> \<in> G.Red_Inf Q G"
+      using \<iota>_in_\<iota>'
+        FL.sat_inf_imp_ground_red_fam_inter[OF satur, unfolded limuls_eq gflimuls_eq, simplified]
       by blast
-    then have \<iota>_red: "G.redundant_infer G \<iota>"
+    then have "G.redundant_infer G \<iota>"
       unfolding G.Red_Inf_def by auto
-
-    have \<gamma>_in_res: "\<gamma> \<in> gd.ord_\<Gamma> Sts"
+    then have \<gamma>_red: "src.redundant_infer G \<gamma>"
+      unfolding \<gamma> by (rule new_redundant_infer_imp_old_redundant_infer)
+    moreover have "\<gamma> \<in> gd.ord_\<Gamma> Sts"
       using \<gamma>_in_inf gd.inferences_from_def by blast
-
-    have \<gamma>_red: "src.redundant_infer G \<gamma>"
-      unfolding \<gamma>
-      apply (rule new_redundant_infer_imp_old_redundant_infer)
-      by (rule \<iota>_red)
-
-    show "\<gamma> \<in> src.Ri Sts G"
-      unfolding src.Ri_def using \<gamma>_in_res \<gamma>_red by auto
+    ultimately show "\<gamma> \<in> src.Ri Sts G"
+      unfolding src.Ri_def by auto
   qed
   then show ?thesis
-    unfolding simps
-    unfolding defs src.saturated_upto_def
-    apply auto
-    by (smt Diff_subset gd.inferences_from_mono subset_eq substitution_ops.grounding_of_clss_def)
+    unfolding G_def clst_eq src.saturated_upto_def
+    by clarsimp (smt Diff_subset gd.inferences_from_mono subset_eq \<G>_Fs_def)
 qed
 
 theorem RP_sound_old_statement:
@@ -1121,13 +1019,12 @@ theorem RP_sound_old_statement:
     deriv: "chain (\<leadsto>) Sts" and
     bot_in: "{#} \<in> clss_of_state (Liminf_state Sts)"
   shows "\<not> satisfiable (grounding_of_state (lhd Sts))"
-  using RP_sound_new_statement[OF deriv bot_in] unfolding F_entails_\<G>_Q_iff by simp
+  using RP_sound_new_statement[OF deriv bot_in] unfolding F_entails_\<G>_Q_iff \<G>_Fs_def by simp
 
-text \<open>FIXME: The theorem below is stated more weakly than the original theorem in RP: The grounding of the
-limit might be a strict subset of the limit of the groundings. See also
+text \<open>The theorem below is stated differently than the original theorem in RP: The grounding of the
+limit might be a strict subset of the limit of the groundings. Because saturation is neither
+monotone nor antimonotone, the two results are incomparable. See also
 @{thm [source] grounding_of_state_Liminf_state_subseteq}.\<close>
-
-thm grounding_of_state_Liminf_state_subseteq
 
 theorem RP_saturated_if_fair_old_statement_altered:
   assumes
@@ -1136,7 +1033,7 @@ theorem RP_saturated_if_fair_old_statement_altered:
     empty_Q0: "Q_of_state (lhd Sts) = {}"
   shows "src.saturated_upto Sts (grounding_of_state (Liminf_state Sts))"
 proof -
-  note fair' = fair_RP_imp_fair[OF chain_not_lnull[OF deriv] fair empty_Q0]
+  note fair' = old_fair_imp_new_fair[OF chain_not_lnull[OF deriv] fair empty_Q0]
   show ?thesis
     apply (rule saturated_imp_saturated_RP[OF _ fair'(2)])
     apply (rule RP_saturated_if_fair_new_statement)
@@ -1153,7 +1050,7 @@ corollary RP_complete_if_fair_old_statement:
   shows "{#} \<in> Q_of_state (Liminf_state Sts)"
   apply (rule RP_complete_if_fair_new_statement)
   apply (rule deriv)
-  apply (rule fair_RP_imp_fair[OF chain_not_lnull[OF deriv] fair empty_Q0])+
+  apply (rule old_fair_imp_new_fair[OF chain_not_lnull[OF deriv] fair empty_Q0])+
   using unsat unfolding F_entails_\<G>_Q_iff by auto
 
 end
