Saturation_Framework/Clausal_Inference_Systems.thy
@@ -11,8 +11,15 @@ theory Clausal_Inference_Systems
     Standard_Redundancy_Criterion
 begin
 
+text \<open>Various results about consequence relations, counterexample-reducing inference systems, and
+the standard redundancy criteria are specialized and customized for clauses as opposed to arbitrary
+formulas.\<close>
+
 
 subsection \<open>Setup\<close>
+
+text \<open>To avoid confusion, we use the symbol \<open>\<TTurnstile>\<close> (with or without subscripts) for the ``models''
+and entailment relations on clauses and \<open>\<Turnstile>\<close> for the abstract concept of consequence.\<close>
 
 abbreviation true_lit_thick :: "'a interp \<Rightarrow> 'a literal \<Rightarrow> bool" (infix "\<TTurnstile>l" 50) where
   "I \<TTurnstile>l L \<equiv> I \<Turnstile>l L"
@@ -40,14 +47,11 @@ abbreviation entails_clss :: "'a clause set \<Rightarrow> 'a clause set \<Righta
 lemma entails_iff_unsatisfiable_single:
   "CC \<TTurnstile>e {E} \<longleftrightarrow> \<not> satisfiable (CC \<union> {{#- L#} |L. L \<in># E})" (is "_ \<longleftrightarrow> _ (_ \<union> ?NegD)")
 proof
-  assume "CC \<TTurnstile>e {E}"
-  then have "\<not> I \<TTurnstile>s CC \<union> ?NegD" for I
-    unfolding true_clss_def true_cls_def true_lit_def if_distribR HOL.if_bool_eq_conj
-    apply (erule_tac x = I in allE)
-    apply (simp add: ball_Un)
-    apply auto
-    using is_pos_neg_not_is_pos apply fastforce
-    using is_pos_neg_not_is_pos by fastforce
+  assume c_ent_e: "CC \<TTurnstile>e {E}"
+  have "\<not> I \<TTurnstile>s CC \<union> ?NegD" for I
+    using c_ent_e[rule_format, of I]
+    unfolding true_clss_def true_cls_def true_lit_def if_distribR if_bool_eq_conj
+    by (fastforce simp: ball_Un is_pos_neg_not_is_pos)
   then show "\<not> satisfiable (CC \<union> ?NegD)"
     by auto
 next
@@ -55,10 +59,8 @@ next
   then have "\<not> I \<TTurnstile>s CC \<union> ?NegD" for I
     by auto
   then show "CC \<TTurnstile>e {E}"
-    unfolding true_clss_def true_cls_def true_lit_def if_distribR HOL.if_bool_eq_conj
-    apply (simp only: ball_Un)
-    apply auto
-    using is_pos_neg_not_is_pos by fastforce
+    unfolding true_clss_def true_cls_def true_lit_def if_distribR if_bool_eq_conj
+    by (fastforce simp: ball_Un is_pos_neg_not_is_pos)
 qed
 
 lemma entails_iff_unsatisfiable:
@@ -75,15 +77,10 @@ qed
 interpretation consequence_relation "{{#}}" "(\<TTurnstile>e)"
 proof
   fix N2 N1 :: "'a clause set"
-  assume "N2 \<subseteq> N1"
-  then show "N1 \<TTurnstile>e N2"
-    using true_clss_mono by blast
-next
-  fix N2 N1 :: "'a clause set"
   assume "\<forall>C \<in> N2. N1 \<TTurnstile>e {C}"
   then show "N1 \<TTurnstile>e N2"
     unfolding true_clss_singleton by (simp add: true_clss_def)
-qed auto
+qed (auto intro: true_clss_mono)
 
 interpretation refute_compact_consequence_relation "{{#}} :: ('a :: wellorder) clause set" "(\<TTurnstile>e)"
   by unfold_locales (use clausal_logic_compact in auto)
@@ -113,16 +110,17 @@ proof
     unfolding CC'_def using d_of fin_e by blast
   moreover have "CC' \<TTurnstile>e EE"
     unfolding entails_iff_unsatisfiable
-    apply (rule ballI)
-    subgoal for E
-      apply (rule unsatisfiable_mono[of "DD_of E"])
-      using d_of[rule_format, THEN conjunct1, of E]
-      unfolding CC'_def
-      apply auto[1]
-      using d_of
-      apply auto
-      done
-    done
+  proof
+    fix E
+    assume e_in: "E \<in> EE"
+
+    have "DD_of E \<subseteq> CC' \<union> {{#- L#} |L. L \<in># E}"
+      using e_in d_of unfolding CC'_def by auto
+    moreover have "\<not> satisfiable (DD_of E)"
+      using e_in d_of by auto
+    ultimately show "\<not> satisfiable (CC' \<union> {{#- L#} |L. L \<in># E})"
+      by (rule unsatisfiable_mono[of "DD_of E"])
+  qed
   ultimately show "\<exists>CC' \<subseteq> CC. finite CC' \<and> CC' \<TTurnstile>e EE"
     by blast
 qed
@@ -136,8 +134,7 @@ definition clss_of_interp :: "'a set \<Rightarrow> 'a literal multiset set" wher
 lemma true_clss_of_interp_iff_equal[simp]: "J \<TTurnstile>s clss_of_interp I \<longleftrightarrow> J = I"
   unfolding clss_of_interp_def true_clss_def true_cls_def true_lit_def by force
 
-lemma entails_iff_models[simp]:
-  "clss_of_interp I \<TTurnstile>e CC \<longleftrightarrow> I \<TTurnstile>s CC"
+lemma entails_iff_models[simp]: "clss_of_interp I \<TTurnstile>e CC \<longleftrightarrow> I \<TTurnstile>s CC"
   by simp
 
 locale clausal_cex_red_inference_system = inference_system Inf
@@ -179,11 +176,7 @@ proof -
     "\<not> clausal_I_of N \<TTurnstile> E" and
     "E < D"
     using clausal_Inf_cex_reducing by metis
-  then show "\<exists>\<iota> \<in> Inf.
-    main_prem_of \<iota> = D \<and> set (side_prems_of \<iota>) \<subseteq> N
-    \<and> I_of N \<TTurnstile>e set (side_prems_of \<iota>)
-    \<and> \<not> I_of N \<TTurnstile>e {concl_of \<iota>}
-    \<and> concl_of \<iota> < D"
+  then show ?thesis
     using snoc_eq_iff_butlast by fastforce
 qed
 
@@ -196,8 +189,7 @@ end
 subsection \<open>Counterexample-Reducing Calculi Equipped with a Standard Redundancy Criterion\<close>
 
 locale clausal_cex_red_calculus_with_std_red_crit =
-  calculus_with_std_red_crit Inf "{{#}}" "(\<TTurnstile>e)" +
-  clausal_cex_red_inference_system Inf clausal_I_of
+  calculus_with_std_red_crit Inf "{{#}}" "(\<TTurnstile>e)" + clausal_cex_red_inference_system Inf clausal_I_of
   for
     Inf :: "('a :: wellorder) clause inference set" and
     clausal_I_of :: "'a clause set \<Rightarrow> 'a set"
